We have:

$$
\begin{eqnarray}
T_{pq} &=&
	\begin{cases}
      a \gets bq + aq + ap \\
      b \gets bp + aq
    \end{cases} \\
    &=&
    \begin{cases}
      a \gets bq + a(p + q) \\
      b \gets bp + aq
    \end{cases}
\end{eqnarray}
$$

and:

$$
\begin{eqnarray}
T^2_{pq}(a, b) &=&
	\begin{cases}
      a \gets q(bp + aq) + q(bq + aq + ap) + p(bq + aq + ap) \\
      b \gets p(bp + aq) + q(bq + aq + ap)
    \end{cases}
\end{eqnarray}
$$

So we need to transform $T^2_{pq}(a, b)$ to something like:

$$
\begin{eqnarray}
T^2_{pq}(a, b) &=&
	\begin{cases}
      a \gets bq' + a(p' + q') \\
      b \gets bp' + aq'
    \end{cases}
\end{eqnarray}
$$

We have:

$$
\begin{eqnarray}
T^2_{pq}(a, b) &=&
	\begin{cases}
      a \gets b(2pq + q^2) + a(2q^2 + 2pq + p^2) \\
      b \gets b(p^2 + q^2) + a(2pq + q^2)
    \end{cases} \\
    &=&
    \begin{cases}
      a \gets b(2pq + q^2) + a((p^2 + q^2) + (2pq + q^2)) \\
      b \gets b(p^2 + q^2) + a(2pq + q^2)
    \end{cases} 
\end{eqnarray}
$$

So it's obvious that $p' = p^2 + q^2$ and $q' = 2pq + q^2$.